@prefix ai: <https://w3id.org/dpv/ai#> .
@prefix dct: <http://purl.org/dc/terms/> .
@prefix dpv: <https://w3id.org/dpv#> .
@prefix owl: <http://www.w3.org/2002/07/owl#> .
@prefix rdfs: <http://www.w3.org/2000/01/rdf-schema#> .
@prefix schema: <https://schema.org/> .
@prefix skos: <http://www.w3.org/2004/02/skos/core#> .
@prefix sw: <http://www.w3.org/2003/06/sw-vocab-status/ns#> .
@prefix vann: <http://purl.org/vocab/vann/> .
@prefix xsd: <http://www.w3.org/2001/XMLSchema#> .

ai:AI a rdfs:Class,
        skos:Concept ;
    dct:created "2024-04-28"^^xsd:date ;
    dct:source "ISO/IEC 22989:2022"@en ;
    rdfs:isDefinedBy ai: ;
    rdfs:subClassOf dpv:Technology ;
    sw:term_status "accepted"@en ;
    skos:broader dpv:Technology ;
    skos:definition "A technical and scientific field devoted to the engineered system that generates outputs such as content, forecasts, recommendations or decisions for a given set of human-defined objectives"@en ;
    skos:inScheme ai:core-classes ;
    skos:prefLabel "Artificial Intelligence (AI)"@en ;
    skos:scopeNote "This concept is a stub"@en .

ai:Capability a rdfs:Class,
        skos:Concept ;
    dct:created "2024-04-28"^^xsd:date ;
    rdfs:isDefinedBy ai: ;
    rdfs:subClassOf ai:AI ;
    sw:term_status "accepted"@en ;
    skos:broader ai:AI ;
    skos:definition "Capability or use of AI to achieve a technical goal or objective"@en ;
    skos:inScheme ai:capabilities-classes ;
    skos:prefLabel "Capability"@en ;
    skos:scopeNote "This concept is a stub"@en .

ai:Measure a rdfs:Class,
        skos:Concept ;
    dct:created "2024-04-28"^^xsd:date ;
    rdfs:isDefinedBy ai: ;
    rdfs:subClassOf dpv:RiskMitigationMeasure ;
    sw:term_status "accepted"@en ;
    skos:broader dpv:RiskMitigationMeasure ;
    skos:definition "Measure to address risk associated with AI Systems"@en ;
    skos:inScheme ai:measures-classes ;
    skos:prefLabel "Measure"@en ;
    skos:scopeNote "This concept is a stub"@en .

ai:Model a rdfs:Class,
        skos:Concept ;
    dct:created "2024-05-17"^^xsd:date ;
    dct:source "ISO/IEC 22989:2022"@en ;
    rdfs:isDefinedBy ai: ;
    rdfs:subClassOf ai:AI ;
    sw:term_status "accepted"@en ;
    skos:broader ai:AI ;
    skos:definition "Physical, mathematical or otherwise logical representation of a system, entity, phenomenon, process or data"@en ;
    skos:inScheme ai:core-classes ;
    skos:prefLabel "Model"@en .

ai:Risk a rdfs:Class,
        skos:Concept ;
    dct:created "2024-04-28"^^xsd:date ;
    rdfs:isDefinedBy ai: ;
    rdfs:subClassOf dpv:Risk ;
    sw:term_status "accepted"@en ;
    skos:broader dpv:Risk ;
    skos:definition "Risk associated with development, use, or operation of AI systems"@en ;
    skos:inScheme ai:risks-classes ;
    skos:prefLabel "Risk"@en ;
    skos:scopeNote "This concept is a stub"@en .

ai:System a rdfs:Class,
        skos:Concept ;
    dct:created "2024-05-17"^^xsd:date ;
    dct:source "OECD, ISO/IEC 22989:2023"@en ;
    rdfs:isDefinedBy ai: ;
    rdfs:subClassOf ai:AI ;
    sw:term_status "accepted"@en ;
    skos:broader ai:AI ;
    skos:definition "OECD 2024 definition: An AI system is a machine-based system that, for explicit or implicit objectives, infers, from the input it receives, how to generate outputs such as predictions, content, recommendations, or decisions that can influence physical or virtual environments. Different AI systems vary in their levels of autonomy and adaptiveness after deployment. ISO/IEC 22989:2023 definition: engineered system that generates outputs such as content, forecasts, recommendations or decisions for a given set of human-defined objectives"@en ;
    skos:inScheme ai:core-classes ;
    skos:prefLabel "System"@en .

ai:Technique a rdfs:Class,
        skos:Concept ;
    dct:created "2024-04-28"^^xsd:date ;
    rdfs:isDefinedBy ai: ;
    rdfs:subClassOf ai:AI ;
    sw:term_status "accepted"@en ;
    skos:broader ai:AI ;
    skos:definition "Techniques for using or applying AI"@en ;
    skos:inScheme ai:techniques-classes ;
    skos:prefLabel "Technique"@en ;
    skos:scopeNote "This concept is a stub"@en .

<https://w3id.org/dpv/ai> a owl:Ontology ;
    dct:conformsTo "http://www.w3.org/2000/01/rdf-schema",
        "http://www.w3.org/2004/02/skos/core" ;
    dct:created "2024-04-28"@en ;
    dct:creator "Delaram Golpayegani"@en,
        "Harshvardhan J. Pandit"@en ;
    dct:description "Extension to the Data Privacy Vocabulary (DPV) providing concepts for representing information about AI technologies"@en ;
    dct:identifier "https://w3id.org/dpv/ai" ;
    dct:license <https://www.w3.org/copyright/document-license-2023/> ;
    dct:title "AI Technology Concepts"@en ;
    vann:preferredNamespacePrefix "ai" ;
    vann:preferredNamespaceUri "https://w3id.org/dpv/ai#" ;
    schema:version "0.1" .

ai:capabilities-classes a skos:ConceptScheme .

ai:measures-classes a skos:ConceptScheme .

ai:risks-classes a skos:ConceptScheme .

ai:techniques-classes a skos:ConceptScheme .

ai:core-classes a skos:ConceptScheme .

