@prefix dct: <http://purl.org/dc/terms/> .
@prefix dpv-owl: <https://w3id.org/dpv/owl#> .
@prefix owl: <http://www.w3.org/2002/07/owl#> .
@prefix pd-owl: <https://w3id.org/dpv/pd/owl#> .
@prefix rdfs: <http://www.w3.org/2000/01/rdf-schema#> .
@prefix schema: <https://schema.org/> .
@prefix skos: <http://www.w3.org/2004/02/skos/core#> .
@prefix sw: <http://www.w3.org/2003/06/sw-vocab-status/ns#> .
@prefix vann: <http://purl.org/vocab/vann/> .
@prefix xsd: <http://www.w3.org/2001/XMLSchema#> .

pd-owl:External a rdfs:Class,
        owl:Class,
        dpv-owl:PersonalData ;
    dct:contributor "Elmar Kiesling; Harshvardhan J. Pandit, Fajar Ekaputra" ;
    dct:created "2019-06-04"^^xsd:date ;
    dct:source "(EnterPrivacy Categories of Personal Information, https://enterprivacy.com/wp-content/uploads/2018/09/Categories-of-Personal-Information.pdf)"@en ;
    rdfs:isDefinedBy pd-owl: ;
    rdfs:subClassOf dpv-owl:PersonalData ;
    sw:term_status "accepted"@en ;
    skos:definition "Information about external characteristics that can be observed"@en ;
    skos:prefLabel "External"@en .

pd-owl:Financial a rdfs:Class,
        owl:Class,
        dpv-owl:PersonalData ;
    dct:contributor "Elmar Kiesling; Harshvardhan J. Pandit, Fajar Ekaputra" ;
    dct:created "2019-06-04"^^xsd:date ;
    dct:source "(EnterPrivacy Categories of Personal Information, https://enterprivacy.com/wp-content/uploads/2018/09/Categories-of-Personal-Information.pdf)"@en ;
    rdfs:isDefinedBy pd-owl: ;
    rdfs:subClassOf dpv-owl:PersonalData ;
    sw:term_status "accepted"@en ;
    skos:definition "Information about finance including monetary characteristics and transactions"@en ;
    skos:prefLabel "Financial"@en ;
    skos:related "svd:Financial"@en .

pd-owl:Historical a rdfs:Class,
        owl:Class,
        dpv-owl:PersonalData ;
    dct:contributor "Elmar Kiesling; Harshvardhan J. Pandit, Fajar Ekaputra" ;
    dct:created "2019-06-04"^^xsd:date ;
    dct:source "(EnterPrivacy Categories of Personal Information, https://enterprivacy.com/wp-content/uploads/2018/09/Categories-of-Personal-Information.pdf)"@en ;
    rdfs:isDefinedBy pd-owl: ;
    rdfs:subClassOf dpv-owl:PersonalData ;
    sw:term_status "accepted"@en ;
    skos:definition "Information about historical data related to or relevant regarding history or past events"@en ;
    skos:prefLabel "Historical"@en .

pd-owl:Household a rdfs:Class,
        owl:Class,
        dpv-owl:PersonalData ;
    dct:contributor "Harshvardhan J. Pandit" ;
    dct:created "2022-06-15"^^xsd:date ;
    rdfs:isDefinedBy pd-owl: ;
    rdfs:subClassOf dpv-owl:PersonalData ;
    sw:term_status "accepted"@en ;
    skos:definition "Information about personal or household activities"@en ;
    skos:prefLabel "Household"@en .

pd-owl:Internal a rdfs:Class,
        owl:Class,
        dpv-owl:PersonalData ;
    dct:contributor "Elmar Kiesling; Harshvardhan J. Pandit, Fajar Ekaputra" ;
    dct:created "2019-06-04"^^xsd:date ;
    dct:source "(EnterPrivacy Categories of Personal Information, https://enterprivacy.com/wp-content/uploads/2018/09/Categories-of-Personal-Information.pdf)"@en ;
    rdfs:isDefinedBy pd-owl: ;
    rdfs:subClassOf dpv-owl:PersonalData ;
    sw:term_status "accepted"@en ;
    skos:definition "Informatoin about internal characteristics that cannot be seen or observed"@en ;
    skos:prefLabel "Internal"@en .

pd-owl:Profile a rdfs:Class,
        owl:Class,
        dpv-owl:PersonalData ;
    dct:contributor "Harshvardhan J. Pandit" ;
    dct:created "2022-06-15"^^xsd:date ;
    rdfs:isDefinedBy pd-owl: ;
    rdfs:subClassOf dpv-owl:PersonalData ;
    sw:term_status "accepted"@en ;
    skos:definition "Profile or user profile is information and representation of characteristics associated with person(s) or group(s)"@en ;
    skos:prefLabel "Profile"@en .

pd-owl:Social a rdfs:Class,
        owl:Class,
        dpv-owl:PersonalData ;
    dct:contributor "Elmar Kiesling; Harshvardhan J. Pandit, Fajar Ekaputra" ;
    dct:created "2019-06-04"^^xsd:date ;
    dct:source "(EnterPrivacy Categories of Personal Information, https://enterprivacy.com/wp-content/uploads/2018/09/Categories-of-Personal-Information.pdf)"@en ;
    rdfs:isDefinedBy pd-owl: ;
    rdfs:subClassOf dpv-owl:PersonalData ;
    sw:term_status "accepted"@en ;
    skos:definition "Information about social aspects such as family, public life, or professional networks."@en ;
    skos:prefLabel "Social"@en .

pd-owl:Tracking a rdfs:Class,
        owl:Class,
        dpv-owl:PersonalData ;
    dct:contributor "Elmar Kiesling; Harshvardhan J. Pandit, Fajar Ekaputra" ;
    dct:created "2019-06-04"^^xsd:date ;
    dct:source "(EnterPrivacy Categories of Personal Information, https://enterprivacy.com/wp-content/uploads/2018/09/Categories-of-Personal-Information.pdf)"@en ;
    rdfs:isDefinedBy pd-owl: ;
    rdfs:subClassOf dpv-owl:PersonalData ;
    sw:term_status "accepted"@en ;
    skos:definition "Information used to track an individual or group e.g. location or email"@en ;
    skos:prefLabel "Tracking"@en .

<https://w3id.org/dpv/pd> a owl:Ontology ;
    dct:conformsTo <http://www.w3.org/2002/07/owl>,
        "http://www.w3.org/2000/01/rdf-schema",
        "http://www.w3.org/2004/02/skos/core" ;
    dct:contributor "Elmar Kiesling",
        "Fajar Ekaputra",
        "Harshvardhan J. Pandit" ;
    dct:created "2022-04-02"@en ;
    dct:creator "Axel Polleres"@en,
        "Harshvardhan J. Pandit"@en ;
    dct:description "Extension to the Data Privacy Vocabulary (DPV) providing additional categories of personal data"@en ;
    dct:hasVersion <https://w3id.org/dpv/pd> ;
    dct:identifier "https://w3id.org/dpv/pd" ;
    dct:license <https://www.w3.org/copyright/document-license-2023/> ;
    dct:modified "2024-01-01"@en ;
    dct:title "Personal Data Categories"@en ;
    vann:preferredNamespacePrefix "pd" ;
    vann:preferredNamespaceUri "https://w3id.org/dpv/pd#" ;
    schema:version "2" .

