@prefix dct: <http://purl.org/dc/terms/> .
@prefix dpv: <https://w3id.org/dpv#> .
@prefix owl: <http://www.w3.org/2002/07/owl#> .
@prefix profile: <http://www.w3.org/ns/dx/prof/> .
@prefix rdf: <http://www.w3.org/1999/02/22-rdf-syntax-ns#> .
@prefix rdfs: <http://www.w3.org/2000/01/rdf-schema#> .
@prefix role: <http://www.w3.org/ns/dx/prof/role/> .
@prefix schema: <https://schema.org/> .
@prefix skos: <http://www.w3.org/2004/02/skos/core#> .
@prefix sw: <http://www.w3.org/2003/06/sw-vocab-status/ns#> .
@prefix vann: <http://purl.org/vocab/vann/> .
@prefix xsd: <http://www.w3.org/2001/XMLSchema#> .

dpv:ControlAssess a rdfs:Class,
        skos:Concept,
        dpv:EntityControl ;
    dct:contributor "Harshvardhan J. Pandit" ;
    dct:created "2024-04-14"^^xsd:date ;
    rdfs:isDefinedBy dpv: ;
    sw:term_status "accepted"@en ;
    skos:broader dpv:EntityControl ;
    skos:definition "Control or measure provided to (another) Entity for assessing information or action"@en ;
    skos:inScheme dpv:entity-control-classes ;
    skos:prefLabel "Control Assess"@en .

dpv:ControlDemonstrate a rdfs:Class,
        skos:Concept,
        dpv:EntityControl ;
    dct:contributor "Harshvardhan J. Pandit" ;
    dct:created "2024-04-14"^^xsd:date ;
    rdfs:isDefinedBy dpv: ;
    sw:term_status "accepted"@en ;
    skos:broader dpv:EntityControl ;
    skos:definition "Control or measure provided to (another) Entity for demonstrating information or action"@en ;
    skos:inScheme dpv:entity-control-classes ;
    skos:prefLabel "Control Demonstrate"@en .

dpv:ControlModify a rdfs:Class,
        skos:Concept,
        dpv:EntityControl ;
    dct:contributor "Harshvardhan J. Pandit" ;
    dct:created "2024-04-14"^^xsd:date ;
    rdfs:isDefinedBy dpv: ;
    sw:term_status "accepted"@en ;
    skos:broader dpv:EntityControl ;
    skos:definition "Control or measure provided to (another) Entity for modifying information or action"@en ;
    skos:inScheme dpv:entity-control-classes ;
    skos:prefLabel "Control Modify"@en ;
    skos:scopeNote "Modify control can be used e.g. to indicate how another entity can modify a previously given consent, or permission, or contract"@en .

dpv:ControlObject a rdfs:Class,
        skos:Concept,
        dpv:EntityControl ;
    dct:contributor "Harshvardhan J. Pandit" ;
    dct:created "2024-04-14"^^xsd:date ;
    rdfs:isDefinedBy dpv: ;
    sw:term_status "accepted"@en ;
    skos:broader dpv:EntityControl ;
    skos:definition "Control or measure provided to (another) Entity for objecting to information or action"@en ;
    skos:inScheme dpv:entity-control-classes ;
    skos:prefLabel "Control Object"@en ;
    skos:scopeNote "Object control can be used e.g. to indicate how another entity can object to processing of data, or use of legitimate interest"@en .

dpv:ControlObtain a rdfs:Class,
        skos:Concept,
        dpv:EntityControl ;
    dct:contributor "Harshvardhan J. Pandit" ;
    dct:created "2024-04-14"^^xsd:date ;
    rdfs:isDefinedBy dpv: ;
    sw:term_status "accepted"@en ;
    skos:broader dpv:EntityControl ;
    skos:definition "Control or measure provided to (another) Entity for obtaining information or action"@en ;
    skos:inScheme dpv:entity-control-classes ;
    skos:prefLabel "Control Obtain"@en .

dpv:ControlProcessChange a rdfs:Class,
        skos:Concept,
        dpv:EntityControl ;
    dct:contributor "Harshvardhan J. Pandit" ;
    dct:created "2024-04-14"^^xsd:date ;
    rdfs:isDefinedBy dpv: ;
    sw:term_status "accepted"@en ;
    skos:broader dpv:EntityControl ;
    skos:definition "Control or measure provided to (another) Entity for processing change in information or action"@en ;
    skos:inScheme dpv:entity-control-classes ;
    skos:prefLabel "Control Process Change"@en .

dpv:ControlProvide a rdfs:Class,
        skos:Concept,
        dpv:EntityControl ;
    dct:contributor "Harshvardhan J. Pandit" ;
    dct:created "2024-04-14"^^xsd:date ;
    rdfs:isDefinedBy dpv: ;
    sw:term_status "accepted"@en ;
    skos:broader dpv:EntityControl ;
    skos:definition "Control or measure provided to (another) Entity for providing information or action"@en ;
    skos:inScheme dpv:entity-control-classes ;
    skos:prefLabel "Control Provide"@en ;
    skos:scopeNote "Provide control can be used e.g. to indicate how another entity will provide consent or establish a contract"@en .

dpv:ControlReaffirm a rdfs:Class,
        skos:Concept,
        dpv:EntityControl ;
    dct:contributor "Harshvardhan J. Pandit" ;
    dct:created "2024-04-14"^^xsd:date ;
    rdfs:isDefinedBy dpv: ;
    sw:term_status "accepted"@en ;
    skos:broader dpv:EntityControl ;
    skos:definition "Control or measure provided to (another) Entity for reaffirming information or action"@en ;
    skos:inScheme dpv:entity-control-classes ;
    skos:prefLabel "Control Reaffirm"@en .

dpv:ControlRecord a rdfs:Class,
        skos:Concept,
        dpv:EntityControl ;
    dct:contributor "Harshvardhan J. Pandit" ;
    dct:created "2024-04-14"^^xsd:date ;
    rdfs:isDefinedBy dpv: ;
    sw:term_status "accepted"@en ;
    skos:broader dpv:EntityControl ;
    skos:definition "Control or measure provided to (another) Entity for recording information or action"@en ;
    skos:inScheme dpv:entity-control-classes ;
    skos:prefLabel "Control Record"@en .

dpv:ControlRetrieve a rdfs:Class,
        skos:Concept,
        dpv:EntityControl ;
    dct:contributor "Harshvardhan J. Pandit" ;
    dct:created "2024-04-14"^^xsd:date ;
    rdfs:isDefinedBy dpv: ;
    sw:term_status "accepted"@en ;
    skos:broader dpv:EntityControl ;
    skos:definition "Control or measure provided to (another) Entity for retrieving information or action"@en ;
    skos:inScheme dpv:entity-control-classes ;
    skos:prefLabel "Control Retrieve"@en .

dpv:ControlTerminate a rdfs:Class,
        skos:Concept,
        dpv:EntityControl ;
    dct:contributor "Harshvardhan J. Pandit" ;
    dct:created "2024-04-14"^^xsd:date ;
    rdfs:isDefinedBy dpv: ;
    sw:term_status "accepted"@en ;
    skos:broader dpv:EntityControl ;
    skos:definition "Control or measure provided to (another) Entity for terminating information or action"@en ;
    skos:inScheme dpv:entity-control-classes ;
    skos:prefLabel "Control Terminate"@en ;
    skos:scopeNote "Terminate control can be used e.g. to indicate how another entity can terminate a contract, or a service"@en .

dpv:ControlWithdraw a rdfs:Class,
        skos:Concept,
        dpv:EntityControl ;
    dct:contributor "Harshvardhan J. Pandit" ;
    dct:created "2024-04-14"^^xsd:date ;
    rdfs:isDefinedBy dpv: ;
    sw:term_status "accepted"@en ;
    skos:broader dpv:EntityControl ;
    skos:definition "Control or measure provided to (another) Entity for withdrawing information or action"@en ;
    skos:inScheme dpv:entity-control-classes ;
    skos:prefLabel "Control Withdraw"@en ;
    skos:scopeNote "Withdraw control can be used e.g. to indicate how another entity can withdraw from a prior agreement, permission, or consent"@en .

dpv:EntityControl a rdfs:Class,
        skos:Concept,
        dpv:TechnicalOrganisationalMeasure ;
    dct:contributor "Harshvardhan J. Pandit" ;
    dct:created "2024-04-14"^^xsd:date ;
    rdfs:isDefinedBy dpv: ;
    sw:term_status "accepted"@en ;
    skos:broader dpv:TechnicalOrganisationalMeasure ;
    skos:definition "Control or measure provided to (another) Entity to enable it to interact or act on some specific information, action, or context"@en ;
    skos:inScheme dpv:entity-control-classes ;
    skos:prefLabel "Entity Control"@en ;
    skos:scopeNote "These are generic controls or measures provided to indicate obtaining, withdrawing, objecting, assessing etc.. For example, to indicate obtaining legal basis of consent, modifying contract, objecting to legitimate interest, or with organisational measures such as reaffirming permissions. To indicate what the control is about, use dct:subject"@en .

<https://w3id.org/dpv> a owl:Ontology,
        profile:Profile ;
    dct:conformsTo "http://www.w3.org/2000/01/rdf-schema",
        "http://www.w3.org/2004/02/skos/core" ;
    dct:contributor "Harshvardhan J. Pandit" ;
    dct:created "2022-08-18"@en ;
    dct:creator "Harshvardhan J. Pandit"@en ;
    dct:description "The Data Privacy Vocabulary (DPV) provides terms (classes and properties) to represent information about processing of personal data, for example - purposes, processing operations, personal data, technical and organisational measures."@en ;
    dct:identifier "https://w3id.org/dpv" ;
    dct:license <https://www.w3.org/copyright/document-license-2023/> ;
    dct:modified "2024-01-01"@en ;
    dct:title "Data Privacy Vocabulary (DPV)"@en ;
    vann:preferredNamespacePrefix "dpv" ;
    vann:preferredNamespaceUri "https://w3id.org/dpv#" ;
    profile:hasResource dpv:serialisation-n3,
        dpv:serialisation-rdf,
        dpv:serialisation-ttl,
        <https://w3id.org/dpv/examples>,
        <https://w3id.org/dpv/guides>,
        <https://w3id.org/dpv/primer> ;
    profile:isProfileOf rdfs:,
        skos: ;
    schema:version "2" .

dpv:serialisation-n3 a profile:ResourceDescriptor ;
    dct:conformsTo <https://www.w3.org/TeamSubmission/n3/> ;
    dct:format <https://www.iana.org/assignments/media-types/text/n3> ;
    dct:title "Data Privacy Vocabulary (DPV) - N3 serialiation" ;
    profile:hasArtifact <https://w3id.org/dpv/dpv.n3> ;
    profile:hasRole role:vocabulary .

dpv:serialisation-rdf a profile:ResourceDescriptor ;
    dct:conformsTo rdf: ;
    dct:format <https://www.iana.org/assignments/media-types/application/rdf+xml> ;
    dct:title "Data Privacy Vocabulary (DPV) - RDF/XML serialiation" ;
    profile:hasArtifact <https://w3id.org/dpv/dpv.rdf> ;
    profile:hasRole role:vocabulary .

dpv:serialisation-ttl a profile:ResourceDescriptor ;
    dct:conformsTo <https://www.w3.org/TR/turtle/> ;
    dct:format <https://www.iana.org/assignments/media-types/text/turtle> ;
    dct:title "Data Privacy Vocabulary (DPV) - Turtle serialiation" ;
    profile:hasArtifact <https://w3id.org/dpv/dpv.ttl> ;
    profile:hasRole role:vocabulary .

<https://w3id.org/dpv/examples> a profile:ResourceDescriptor ;
    dct:conformsTo <https://www.w3.org/TR/html/> ;
    dct:format <https://www.iana.org/assignments/media-types/text/html> ;
    dct:title "Examples for Data Privacy Vocabulary" ;
    profile:hasArtifact <https://w3id.org/dpv/examples> ;
    profile:hasRole role:guidance .

<https://w3id.org/dpv/guides> a profile:ResourceDescriptor ;
    dct:conformsTo <https://www.w3.org/TR/html/> ;
    dct:format <https://www.iana.org/assignments/media-types/text/html> ;
    dct:title "Guides for Data Privacy Vocabulary" ;
    profile:hasArtifact <https://w3id.org/dpv/guides> ;
    profile:hasRole role:guidance .

<https://w3id.org/dpv/primer> a profile:ResourceDescriptor ;
    dct:conformsTo <https://www.w3.org/TR/html/> ;
    dct:format <https://www.iana.org/assignments/media-types/text/html> ;
    dct:title "Primer for Data Privacy Vocabulary" ;
    profile:hasArtifact <https://w3id.org/dpv/primer> ;
    profile:hasRole role:guidance .

dpv:entity-control-classes a skos:ConceptScheme .

