<?xml version="1.0" encoding="utf-8"?>
<rdf:RDF
   xmlns:dct="http://purl.org/dc/terms/"
   xmlns:rdf="http://www.w3.org/1999/02/22-rdf-syntax-ns#"
   xmlns:rdfs="http://www.w3.org/2000/01/rdf-schema#"
   xmlns:schema="https://schema.org/"
   xmlns:skos="http://www.w3.org/2004/02/skos/core#"
   xmlns:sw="http://www.w3.org/2003/06/sw-vocab-status/ns#"
   xmlns:vann="http://purl.org/vocab/vann/"
>
  <rdf:Description rdf:about="https://w3id.org/dpv/owl#ControlObtain">
    <skos:prefLabel xml:lang="en">Control Obtain</skos:prefLabel>
    <skos:definition xml:lang="en">Control or measure provided to (another) Entity for obtaining information or action</skos:definition>
    <dct:created rdf:datatype="http://www.w3.org/2001/XMLSchema#date">2024-04-14</dct:created>
    <dct:contributor>Harshvardhan J. Pandit</dct:contributor>
    <rdf:type rdf:resource="http://www.w3.org/2000/01/rdf-schema#Class"/>
    <rdf:type rdf:resource="https://w3id.org/dpv/owl#EntityControl"/>
    <rdf:type rdf:resource="http://www.w3.org/2002/07/owl#Class"/>
    <rdfs:isDefinedBy rdf:resource="https://w3id.org/dpv/owl#"/>
    <sw:term_status xml:lang="en">accepted</sw:term_status>
    <rdfs:subClassOf rdf:resource="https://w3id.org/dpv/owl#EntityControl"/>
  </rdf:Description>
  <rdf:Description rdf:about="https://w3id.org/dpv">
    <dct:conformsTo>http://www.w3.org/2004/02/skos/core</dct:conformsTo>
    <dct:conformsTo>http://www.w3.org/2000/01/rdf-schema</dct:conformsTo>
    <dct:conformsTo rdf:resource="http://www.w3.org/2002/07/owl"/>
    <vann:preferredNamespaceUri>https://w3id.org/dpv#</vann:preferredNamespaceUri>
    <dct:title xml:lang="en">Data Privacy Vocabulary (DPV)</dct:title>
    <dct:contributor>Harshvardhan J. Pandit</dct:contributor>
    <dct:modified xml:lang="en">2024-01-01</dct:modified>
    <rdf:type rdf:resource="http://www.w3.org/2002/07/owl#Ontology"/>
    <dct:creator xml:lang="en">Harshvardhan J. Pandit</dct:creator>
    <dct:identifier>https://w3id.org/dpv</dct:identifier>
    <schema:version>2</schema:version>
    <vann:preferredNamespacePrefix>dpv</vann:preferredNamespacePrefix>
    <dct:created xml:lang="en">2022-08-18</dct:created>
    <dct:license rdf:resource="https://www.w3.org/copyright/document-license-2023/"/>
    <dct:description xml:lang="en">The Data Privacy Vocabulary (DPV) provides terms (classes and properties) to represent information about processing of personal data, for example - purposes, processing operations, personal data, technical and organisational measures.</dct:description>
    <dct:hasVersion rdf:resource="https://w3id.org/dpv"/>
  </rdf:Description>
  <rdf:Description rdf:about="https://w3id.org/dpv/owl#ControlRetrieve">
    <dct:contributor>Harshvardhan J. Pandit</dct:contributor>
    <rdf:type rdf:resource="http://www.w3.org/2000/01/rdf-schema#Class"/>
    <rdf:type rdf:resource="https://w3id.org/dpv/owl#EntityControl"/>
    <rdf:type rdf:resource="http://www.w3.org/2002/07/owl#Class"/>
    <skos:prefLabel xml:lang="en">Control Retrieve</skos:prefLabel>
    <skos:definition xml:lang="en">Control or measure provided to (another) Entity for retrieving information or action</skos:definition>
    <sw:term_status xml:lang="en">accepted</sw:term_status>
    <dct:created rdf:datatype="http://www.w3.org/2001/XMLSchema#date">2024-04-14</dct:created>
    <rdfs:isDefinedBy rdf:resource="https://w3id.org/dpv/owl#"/>
    <rdfs:subClassOf rdf:resource="https://w3id.org/dpv/owl#EntityControl"/>
  </rdf:Description>
  <rdf:Description rdf:about="https://w3id.org/dpv/owl#ControlDemonstrate">
    <skos:prefLabel xml:lang="en">Control Demonstrate</skos:prefLabel>
    <dct:contributor>Harshvardhan J. Pandit</dct:contributor>
    <skos:definition xml:lang="en">Control or measure provided to (another) Entity for demonstrating information or action</skos:definition>
    <sw:term_status xml:lang="en">accepted</sw:term_status>
    <dct:created rdf:datatype="http://www.w3.org/2001/XMLSchema#date">2024-04-14</dct:created>
    <rdf:type rdf:resource="http://www.w3.org/2000/01/rdf-schema#Class"/>
    <rdf:type rdf:resource="https://w3id.org/dpv/owl#EntityControl"/>
    <rdf:type rdf:resource="http://www.w3.org/2002/07/owl#Class"/>
    <rdfs:isDefinedBy rdf:resource="https://w3id.org/dpv/owl#"/>
    <rdfs:subClassOf rdf:resource="https://w3id.org/dpv/owl#EntityControl"/>
  </rdf:Description>
  <rdf:Description rdf:about="https://w3id.org/dpv/owl#ControlAssess">
    <skos:prefLabel xml:lang="en">Control Assess</skos:prefLabel>
    <skos:definition xml:lang="en">Control or measure provided to (another) Entity for assessing information or action</skos:definition>
    <rdf:type rdf:resource="https://w3id.org/dpv/owl#EntityControl"/>
    <rdf:type rdf:resource="http://www.w3.org/2000/01/rdf-schema#Class"/>
    <rdf:type rdf:resource="http://www.w3.org/2002/07/owl#Class"/>
    <rdfs:isDefinedBy rdf:resource="https://w3id.org/dpv/owl#"/>
    <dct:contributor>Harshvardhan J. Pandit</dct:contributor>
    <sw:term_status xml:lang="en">accepted</sw:term_status>
    <dct:created rdf:datatype="http://www.w3.org/2001/XMLSchema#date">2024-04-14</dct:created>
    <rdfs:subClassOf rdf:resource="https://w3id.org/dpv/owl#EntityControl"/>
  </rdf:Description>
  <rdf:Description rdf:about="https://w3id.org/dpv/owl#ControlProcessChange">
    <sw:term_status xml:lang="en">accepted</sw:term_status>
    <skos:definition xml:lang="en">Control or measure provided to (another) Entity for processing change in information or action</skos:definition>
    <rdf:type rdf:resource="http://www.w3.org/2000/01/rdf-schema#Class"/>
    <rdf:type rdf:resource="https://w3id.org/dpv/owl#EntityControl"/>
    <rdf:type rdf:resource="http://www.w3.org/2002/07/owl#Class"/>
    <rdfs:isDefinedBy rdf:resource="https://w3id.org/dpv/owl#"/>
    <dct:created rdf:datatype="http://www.w3.org/2001/XMLSchema#date">2024-04-14</dct:created>
    <skos:prefLabel xml:lang="en">Control Process Change</skos:prefLabel>
    <dct:contributor>Harshvardhan J. Pandit</dct:contributor>
    <rdfs:subClassOf rdf:resource="https://w3id.org/dpv/owl#EntityControl"/>
  </rdf:Description>
  <rdf:Description rdf:about="https://w3id.org/dpv/owl#ControlReaffirm">
    <dct:created rdf:datatype="http://www.w3.org/2001/XMLSchema#date">2024-04-14</dct:created>
    <dct:contributor>Harshvardhan J. Pandit</dct:contributor>
    <skos:prefLabel xml:lang="en">Control Reaffirm</skos:prefLabel>
    <sw:term_status xml:lang="en">accepted</sw:term_status>
    <rdf:type rdf:resource="http://www.w3.org/2000/01/rdf-schema#Class"/>
    <rdf:type rdf:resource="https://w3id.org/dpv/owl#EntityControl"/>
    <rdf:type rdf:resource="http://www.w3.org/2002/07/owl#Class"/>
    <skos:definition xml:lang="en">Control or measure provided to (another) Entity for reaffirming information or action</skos:definition>
    <rdfs:isDefinedBy rdf:resource="https://w3id.org/dpv/owl#"/>
    <rdfs:subClassOf rdf:resource="https://w3id.org/dpv/owl#EntityControl"/>
  </rdf:Description>
  <rdf:Description rdf:about="https://w3id.org/dpv/owl#EntityControl">
    <rdf:type rdf:resource="https://w3id.org/dpv/owl#TechnicalOrganisationalMeasure"/>
    <rdf:type rdf:resource="http://www.w3.org/2000/01/rdf-schema#Class"/>
    <rdf:type rdf:resource="http://www.w3.org/2002/07/owl#Class"/>
    <dct:created rdf:datatype="http://www.w3.org/2001/XMLSchema#date">2024-04-14</dct:created>
    <skos:prefLabel xml:lang="en">Entity Control</skos:prefLabel>
    <rdfs:isDefinedBy rdf:resource="https://w3id.org/dpv/owl#"/>
    <dct:contributor>Harshvardhan J. Pandit</dct:contributor>
    <skos:definition xml:lang="en">Control or measure provided to (another) Entity to enable it to interact or act on some specific information, action, or context</skos:definition>
    <skos:scopeNote xml:lang="en">These are generic controls or measures provided to indicate obtaining, withdrawing, objecting, assessing etc.. For example, to indicate obtaining legal basis of consent, modifying contract, objecting to legitimate interest, or with organisational measures such as reaffirming permissions. To indicate what the control is about, use dct:subject</skos:scopeNote>
    <sw:term_status xml:lang="en">accepted</sw:term_status>
    <rdfs:subClassOf rdf:resource="https://w3id.org/dpv/owl#TechnicalOrganisationalMeasure"/>
  </rdf:Description>
  <rdf:Description rdf:about="https://w3id.org/dpv/owl#ControlTerminate">
    <dct:created rdf:datatype="http://www.w3.org/2001/XMLSchema#date">2024-04-14</dct:created>
    <rdf:type rdf:resource="http://www.w3.org/2000/01/rdf-schema#Class"/>
    <rdf:type rdf:resource="https://w3id.org/dpv/owl#EntityControl"/>
    <rdf:type rdf:resource="http://www.w3.org/2002/07/owl#Class"/>
    <rdfs:isDefinedBy rdf:resource="https://w3id.org/dpv/owl#"/>
    <dct:contributor>Harshvardhan J. Pandit</dct:contributor>
    <skos:scopeNote xml:lang="en">Terminate control can be used e.g. to indicate how another entity can terminate a contract, or a service</skos:scopeNote>
    <skos:prefLabel xml:lang="en">Control Terminate</skos:prefLabel>
    <skos:definition xml:lang="en">Control or measure provided to (another) Entity for terminating information or action</skos:definition>
    <sw:term_status xml:lang="en">accepted</sw:term_status>
    <rdfs:subClassOf rdf:resource="https://w3id.org/dpv/owl#EntityControl"/>
  </rdf:Description>
  <rdf:Description rdf:about="https://w3id.org/dpv/owl#ControlObject">
    <rdf:type rdf:resource="http://www.w3.org/2000/01/rdf-schema#Class"/>
    <rdf:type rdf:resource="https://w3id.org/dpv/owl#EntityControl"/>
    <rdf:type rdf:resource="http://www.w3.org/2002/07/owl#Class"/>
    <skos:definition xml:lang="en">Control or measure provided to (another) Entity for objecting to information or action</skos:definition>
    <rdfs:isDefinedBy rdf:resource="https://w3id.org/dpv/owl#"/>
    <dct:contributor>Harshvardhan J. Pandit</dct:contributor>
    <sw:term_status xml:lang="en">accepted</sw:term_status>
    <dct:created rdf:datatype="http://www.w3.org/2001/XMLSchema#date">2024-04-14</dct:created>
    <skos:scopeNote xml:lang="en">Object control can be used e.g. to indicate how another entity can object to processing of data, or use of legitimate interest</skos:scopeNote>
    <skos:prefLabel xml:lang="en">Control Object</skos:prefLabel>
    <rdfs:subClassOf rdf:resource="https://w3id.org/dpv/owl#EntityControl"/>
  </rdf:Description>
  <rdf:Description rdf:about="https://w3id.org/dpv/owl#ControlModify">
    <rdfs:isDefinedBy rdf:resource="https://w3id.org/dpv/owl#"/>
    <rdf:type rdf:resource="http://www.w3.org/2000/01/rdf-schema#Class"/>
    <rdf:type rdf:resource="https://w3id.org/dpv/owl#EntityControl"/>
    <rdf:type rdf:resource="http://www.w3.org/2002/07/owl#Class"/>
    <dct:contributor>Harshvardhan J. Pandit</dct:contributor>
    <skos:prefLabel xml:lang="en">Control Modify</skos:prefLabel>
    <sw:term_status xml:lang="en">accepted</sw:term_status>
    <skos:definition xml:lang="en">Control or measure provided to (another) Entity for modifying information or action</skos:definition>
    <skos:scopeNote xml:lang="en">Modify control can be used e.g. to indicate how another entity can modify a previously given consent, or permission, or contract</skos:scopeNote>
    <dct:created rdf:datatype="http://www.w3.org/2001/XMLSchema#date">2024-04-14</dct:created>
    <rdfs:subClassOf rdf:resource="https://w3id.org/dpv/owl#EntityControl"/>
  </rdf:Description>
  <rdf:Description rdf:about="https://w3id.org/dpv/owl#ControlRecord">
    <dct:created rdf:datatype="http://www.w3.org/2001/XMLSchema#date">2024-04-14</dct:created>
    <skos:definition xml:lang="en">Control or measure provided to (another) Entity for recording information or action</skos:definition>
    <dct:contributor>Harshvardhan J. Pandit</dct:contributor>
    <skos:prefLabel xml:lang="en">Control Record</skos:prefLabel>
    <rdf:type rdf:resource="http://www.w3.org/2000/01/rdf-schema#Class"/>
    <rdf:type rdf:resource="https://w3id.org/dpv/owl#EntityControl"/>
    <rdf:type rdf:resource="http://www.w3.org/2002/07/owl#Class"/>
    <sw:term_status xml:lang="en">accepted</sw:term_status>
    <rdfs:isDefinedBy rdf:resource="https://w3id.org/dpv/owl#"/>
    <rdfs:subClassOf rdf:resource="https://w3id.org/dpv/owl#EntityControl"/>
  </rdf:Description>
  <rdf:Description rdf:about="https://w3id.org/dpv/owl#ControlProvide">
    <dct:contributor>Harshvardhan J. Pandit</dct:contributor>
    <skos:definition xml:lang="en">Control or measure provided to (another) Entity for providing information or action</skos:definition>
    <sw:term_status xml:lang="en">accepted</sw:term_status>
    <dct:created rdf:datatype="http://www.w3.org/2001/XMLSchema#date">2024-04-14</dct:created>
    <skos:prefLabel xml:lang="en">Control Provide</skos:prefLabel>
    <rdf:type rdf:resource="http://www.w3.org/2000/01/rdf-schema#Class"/>
    <rdf:type rdf:resource="https://w3id.org/dpv/owl#EntityControl"/>
    <rdf:type rdf:resource="http://www.w3.org/2002/07/owl#Class"/>
    <skos:scopeNote xml:lang="en">Provide control can be used e.g. to indicate how another entity will provide consent or establish a contract</skos:scopeNote>
    <rdfs:isDefinedBy rdf:resource="https://w3id.org/dpv/owl#"/>
    <rdfs:subClassOf rdf:resource="https://w3id.org/dpv/owl#EntityControl"/>
  </rdf:Description>
  <rdf:Description rdf:about="https://w3id.org/dpv/owl#ControlWithdraw">
    <skos:prefLabel xml:lang="en">Control Withdraw</skos:prefLabel>
    <dct:created rdf:datatype="http://www.w3.org/2001/XMLSchema#date">2024-04-14</dct:created>
    <rdf:type rdf:resource="http://www.w3.org/2000/01/rdf-schema#Class"/>
    <rdf:type rdf:resource="https://w3id.org/dpv/owl#EntityControl"/>
    <rdf:type rdf:resource="http://www.w3.org/2002/07/owl#Class"/>
    <skos:scopeNote xml:lang="en">Withdraw control can be used e.g. to indicate how another entity can withdraw from a prior agreement, permission, or consent</skos:scopeNote>
    <rdfs:isDefinedBy rdf:resource="https://w3id.org/dpv/owl#"/>
    <dct:contributor>Harshvardhan J. Pandit</dct:contributor>
    <skos:definition xml:lang="en">Control or measure provided to (another) Entity for withdrawing information or action</skos:definition>
    <sw:term_status xml:lang="en">accepted</sw:term_status>
    <rdfs:subClassOf rdf:resource="https://w3id.org/dpv/owl#EntityControl"/>
  </rdf:Description>
</rdf:RDF>
