@prefix dct: <http://purl.org/dc/terms/> .
@prefix dpv-owl: <https://w3id.org/dpv/owl#> .
@prefix owl: <http://www.w3.org/2002/07/owl#> .
@prefix profile: <http://www.w3.org/ns/dx/prof/> .
@prefix rdf: <http://www.w3.org/1999/02/22-rdf-syntax-ns#> .
@prefix rdfs: <http://www.w3.org/2000/01/rdf-schema#> .
@prefix role: <http://www.w3.org/ns/dx/prof/role/> .
@prefix schema: <https://schema.org/> .
@prefix skos: <http://www.w3.org/2004/02/skos/core#> .
@prefix sw: <http://www.w3.org/2003/06/sw-vocab-status/ns#> .
@prefix vann: <http://purl.org/vocab/vann/> .
@prefix xsd: <http://www.w3.org/2001/XMLSchema#> .

dpv-owl:EnvironmentalProtection a rdfs:Class,
        owl:Class,
        dpv-owl:PhysicalMeasure ;
    dct:contributor "Harshvardhan J. Pandit" ;
    dct:created "2024-04-14"^^xsd:date ;
    dct:source "NIST SP 800-13"@en ;
    rdfs:isDefinedBy dpv-owl: ;
    rdfs:subClassOf dpv-owl:PhysicalMeasure ;
    sw:term_status "accepted"@en ;
    skos:definition "Physical protection against environmental threats such as fire, floods, storms, etc."@en ;
    skos:prefLabel "Environmental Protection"@en .

dpv-owl:PhysicalAccessControlMethod a rdfs:Class,
        owl:Class,
        dpv-owl:PhysicalMeasure ;
    dct:contributor "Georg P. Krog" ;
    dct:created "2022-06-15"^^xsd:date ;
    dct:source "NIST SP 800-12"@en ;
    rdfs:isDefinedBy dpv-owl: ;
    rdfs:subClassOf dpv-owl:AccessControlMethod ;
    sw:term_status "accepted"@en ;
    skos:definition "Access control applied for physical access e.g. premises or equipment"@en ;
    skos:prefLabel "Physical Access Control Method"@en .

dpv-owl:PhysicalAuthentication a rdfs:Class,
        owl:Class,
        dpv-owl:PhysicalMeasure ;
    dct:contributor "Harshvardhan J. Pandit" ;
    dct:created "2024-04-14"^^xsd:date ;
    dct:source "NIST SP 800-15"@en ;
    rdfs:isDefinedBy dpv-owl: ;
    rdfs:subClassOf dpv-owl:PhysicalMeasure ;
    sw:term_status "accepted"@en ;
    skos:definition "Physical implementation of authentication e.g. by matching the person to their ID card"@en ;
    skos:prefLabel "Physical Authentication"@en .

dpv-owl:PhysicalAuthorisation a rdfs:Class,
        owl:Class,
        dpv-owl:PhysicalMeasure ;
    dct:contributor "Harshvardhan J. Pandit" ;
    dct:created "2024-04-14"^^xsd:date ;
    dct:source "NIST SP 800-16"@en ;
    rdfs:isDefinedBy dpv-owl: ;
    rdfs:subClassOf dpv-owl:PhysicalMeasure ;
    sw:term_status "accepted"@en ;
    skos:definition "Physical implementation of authorisation e.g. by stamping a visitor pass"@en ;
    skos:prefLabel "Physical Authorisation"@en .

dpv-owl:PhysicalDeviceSecurity a rdfs:Class,
        owl:Class,
        dpv-owl:PhysicalMeasure ;
    dct:contributor "Harshvardhan J. Pandit" ;
    dct:created "2024-04-14"^^xsd:date ;
    dct:source "NIST SP 800-19"@en ;
    rdfs:isDefinedBy dpv-owl: ;
    rdfs:subClassOf dpv-owl:PhysicalMeasure ;
    sw:term_status "accepted"@en ;
    skos:definition "Physical protection for devices and equipment"@en ;
    skos:prefLabel "Physical Device Security"@en .

dpv-owl:PhysicalInterceptionProtection a rdfs:Class,
        owl:Class,
        dpv-owl:PhysicalMeasure ;
    dct:contributor "Harshvardhan J. Pandit" ;
    dct:created "2024-04-14"^^xsd:date ;
    dct:source "NIST SP 800-20"@en ;
    rdfs:isDefinedBy dpv-owl: ;
    rdfs:subClassOf dpv-owl:PhysicalMeasure ;
    sw:term_status "accepted"@en ;
    skos:definition "Physical protection against interception e.g. by posting a guard"@en ;
    skos:prefLabel "Physical Interception Protection"@en .

dpv-owl:PhysicalInterruptionProtection a rdfs:Class,
        owl:Class,
        dpv-owl:PhysicalMeasure ;
    dct:contributor "Harshvardhan J. Pandit" ;
    dct:created "2024-04-14"^^xsd:date ;
    dct:source "NIST SP 800-18"@en ;
    rdfs:isDefinedBy dpv-owl: ;
    rdfs:subClassOf dpv-owl:PhysicalMeasure ;
    sw:term_status "accepted"@en ;
    skos:definition "Physical protection against interruptions e.g. electrical supply interruption"@en ;
    skos:prefLabel "Physical Interruption Protection"@en .

dpv-owl:PhysicalNetworkSecurity a rdfs:Class,
        owl:Class,
        dpv-owl:PhysicalMeasure ;
    dct:contributor "Harshvardhan J. Pandit" ;
    dct:created "2024-04-14"^^xsd:date ;
    dct:source "NIST SP 800-17"@en ;
    rdfs:isDefinedBy dpv-owl: ;
    rdfs:subClassOf dpv-owl:PhysicalMeasure ;
    sw:term_status "accepted"@en ;
    skos:definition "Physical protection for networks and networking related infrastructure e.g. by isolating networking equipments"@en ;
    skos:prefLabel "Physical Network Security"@en .

dpv-owl:PhysicalSecureStorage a rdfs:Class,
        owl:Class,
        dpv-owl:PhysicalMeasure ;
    dct:contributor "Harshvardhan J. Pandit" ;
    dct:created "2024-04-14"^^xsd:date ;
    dct:source "NIST SP 800-171"@en ;
    rdfs:isDefinedBy dpv-owl: ;
    rdfs:subClassOf dpv-owl:PhysicalMeasure ;
    sw:term_status "accepted"@en ;
    skos:definition "Physical protection for storage of information or equipment e.g. secure storage for files"@en ;
    skos:prefLabel "Physical Secure Storage"@en .

dpv-owl:PhysicalSupplySecurity a rdfs:Class,
        owl:Class,
        dpv-owl:PhysicalMeasure ;
    dct:contributor "Harshvardhan J. Pandit" ;
    dct:created "2024-04-14"^^xsd:date ;
    dct:source "NIST SP 800-14"@en ;
    rdfs:isDefinedBy dpv-owl: ;
    rdfs:subClassOf dpv-owl:PhysicalMeasure ;
    sw:term_status "accepted"@en ;
    skos:definition "Physically securing the supply of resources"@en ;
    skos:prefLabel "Physical Supply Security"@en .

dpv-owl:PhysicalSurveillance a rdfs:Class,
        owl:Class,
        dpv-owl:PhysicalMeasure ;
    dct:contributor "Harshvardhan J. Pandit" ;
    dct:created "2024-04-14"^^xsd:date ;
    dct:source "NIST SP 800-171"@en ;
    rdfs:isDefinedBy dpv-owl: ;
    rdfs:subClassOf dpv-owl:PhysicalMeasure ;
    sw:term_status "accepted"@en ;
    skos:definition "Physically monitoring areas via surveillance"@en ;
    skos:prefLabel "Physical Surveillance"@en .

dpv-owl:serialisation-jsonld a profile:ResourceDescriptor ;
    dct:conformsTo <http://www.w3.org/2002/07/owl>,
        <https://www.w3.org/TR/json-ld11/> ;
    dct:format <https://www.iana.org/assignments/media-types/application/ld+json> ;
    dct:hasVersion <https://w3id.org/dpv> ;
    dct:title "Data Privacy Vocabulary (DPV) - JSON-LD serialiation" ;
    profile:hasArtifact <https://w3id.org/dpv/dpv.jsonld> ;
    profile:hasRole role:vocabulary .

dpv-owl:serialisation-n3 a profile:ResourceDescriptor ;
    dct:conformsTo <http://www.w3.org/2002/07/owl>,
        <https://www.w3.org/TeamSubmission/n3/> ;
    dct:format <https://www.iana.org/assignments/media-types/text/n3> ;
    dct:hasVersion <https://w3id.org/dpv> ;
    dct:title "Data Privacy Vocabulary (DPV) - N3 serialiation" ;
    profile:hasArtifact <https://w3id.org/dpv/dpv.n3> ;
    profile:hasRole role:vocabulary .

dpv-owl:serialisation-rdf a profile:ResourceDescriptor ;
    dct:conformsTo rdf:,
        <http://www.w3.org/2002/07/owl> ;
    dct:format <https://www.iana.org/assignments/media-types/application/rdf+xml> ;
    dct:hasVersion <https://w3id.org/dpv> ;
    dct:title "Data Privacy Vocabulary (DPV) - RDF/XML serialiation" ;
    profile:hasArtifact <https://w3id.org/dpv/dpv.rdf> ;
    profile:hasRole role:vocabulary .

dpv-owl:serialisation-ttl a profile:ResourceDescriptor ;
    dct:conformsTo <http://www.w3.org/2002/07/owl>,
        <https://www.w3.org/TR/turtle/> ;
    dct:format <https://www.iana.org/assignments/media-types/text/turtle> ;
    dct:hasVersion <https://w3id.org/dpv> ;
    dct:title "Data Privacy Vocabulary (DPV) - Turtle serialiation" ;
    profile:hasArtifact <https://w3id.org/dpv/dpv.ttl> ;
    profile:hasRole role:vocabulary .

<https://w3id.org/dpv/examples> dct:conformsTo <http://www.w3.org/2002/07/owl>,
        <https://www.w3.org/TR/html/> ;
    dct:format <https://www.iana.org/assignments/media-types/text/html> ;
    dct:hasVersion <https://w3id.org/dpv> ;
    dct:title "Examples for Data Privacy Vocabulary" ;
    profile:hasArtifact <https://w3id.org/dpv/examples> ;
    profile:hasRole role:guidance .

<https://w3id.org/dpv/guides> dct:conformsTo <http://www.w3.org/2002/07/owl>,
        <https://www.w3.org/TR/html/> ;
    dct:format <https://www.iana.org/assignments/media-types/text/html> ;
    dct:hasVersion <https://w3id.org/dpv> ;
    dct:title "Guides for Data Privacy Vocabulary" ;
    profile:hasArtifact <https://w3id.org/dpv/guides> ;
    profile:hasRole role:guidance .

<https://w3id.org/dpv/primer> dct:conformsTo <http://www.w3.org/2002/07/owl>,
        <https://www.w3.org/TR/html/> ;
    dct:format <https://www.iana.org/assignments/media-types/text/html> ;
    dct:hasVersion <https://w3id.org/dpv> ;
    dct:title "Primer for Data Privacy Vocabulary" ;
    profile:hasArtifact <https://w3id.org/dpv/primer> ;
    profile:hasRole role:guidance .

<https://w3id.org/dpv> a owl:Ontology,
        profile:Profile ;
    dct:conformsTo <http://www.w3.org/2002/07/owl>,
        "http://www.w3.org/2000/01/rdf-schema",
        "http://www.w3.org/2004/02/skos/core" ;
    dct:contributor "Georg P. Krog",
        "Harshvardhan J. Pandit" ;
    dct:created "2022-08-18"@en ;
    dct:creator "Harshvardhan J. Pandit"@en ;
    dct:description "The Data Privacy Vocabulary (DPV) provides terms (classes and properties) to represent information about processing of personal data, for example - purposes, processing operations, personal data, technical and organisational measures."@en ;
    dct:hasVersion <https://w3id.org/dpv> ;
    dct:identifier "https://w3id.org/dpv" ;
    dct:license <https://www.w3.org/copyright/document-license-2023/> ;
    dct:modified "2024-01-01"@en ;
    dct:title "Data Privacy Vocabulary (DPV)"@en ;
    vann:preferredNamespacePrefix "dpv" ;
    vann:preferredNamespaceUri "https://w3id.org/dpv#" ;
    profile:hasResource <https://w3id.org/dpv/examples>,
        <https://w3id.org/dpv/guides>,
        dpv-owl:serialisation-jsonld,
        dpv-owl:serialisation-n3,
        dpv-owl:serialisation-rdf,
        dpv-owl:serialisation-ttl,
        <https://w3id.org/dpv/primer> ;
    profile:isProfileOf <http://www.w3.org/2002/07/owl>,
        <https://w3id.org/dpv> ;
    schema:version "2" .

