@prefix dcam: <http://purl.org/dc/dcam/> .
@prefix dct: <http://purl.org/dc/terms/> .
@prefix dex: <https://w3id.org/dpv/examples#> .
@prefix dpv: <https://w3id.org/dpv#> .
@prefix owl: <http://www.w3.org/2002/07/owl#> .
@prefix profile: <http://www.w3.org/ns/dx/prof/> .
@prefix rdf: <http://www.w3.org/1999/02/22-rdf-syntax-ns#> .
@prefix rdfs: <http://www.w3.org/2000/01/rdf-schema#> .
@prefix role: <http://www.w3.org/ns/dx/prof/role/> .
@prefix schema: <https://schema.org/> .
@prefix skos: <http://www.w3.org/2004/02/skos/core#> .
@prefix sw: <http://www.w3.org/2003/06/sw-vocab-status/ns#> .
@prefix vann: <http://purl.org/vocab/vann/> .
@prefix xsd: <http://www.w3.org/2001/XMLSchema#> .

dpv:NonPersonalDataProcess a rdfs:Class,
        skos:Concept ;
    dct:contributor "Harshvardhan J. Pandit" ;
    rdfs:isDefinedBy dpv: ;
    rdfs:subClassOf dpv:Process ;
    sw:term_status "accepted"@en ;
    skos:broader dpv:Process ;
    skos:definition "An action, activity, or method involving non-personal data, and asserting that no personal data is involved"@en ;
    skos:inScheme dpv:process-classes ;
    skos:prefLabel "Non-Personal Data Process"@en ;
    skos:scopeNote "Use of personal data within NonPersonalDataProcess should be considered a violation of the explicit constraint that no personal data is involved."@en .

dpv:PersonalDataHandling a rdfs:Class,
        skos:Concept ;
    dct:contributor "Axel Polleres, Javier Fernández" ;
    dct:created "2019-04-05"^^xsd:date ;
    dct:modified "2023-12-10"^^xsd:date ;
    vann:example dex:E0007,
        dex:E0008,
        dex:E0014,
        dex:E0018,
        dex:E0019,
        dex:E0020,
        dex:E0022,
        dex:E0028 ;
    rdfs:isDefinedBy dpv: ;
    rdfs:subClassOf dpv:Process ;
    sw:term_status "sunset"@en ;
    skos:broader dpv:Process ;
    skos:definition "An abstract concept describing 'personal data handling'"@en ;
    skos:inScheme dpv:process-classes ;
    skos:prefLabel "Personal Data Handling"@en ;
    skos:scopeNote "This concept will be deprecated in future updates. It is recommended to use dpv:PersonalDataProcess as the equivalent alternative which is better aligned with legal and operational terminology."@en .

dpv:PersonalDataProcess a rdfs:Class,
        skos:Concept ;
    dct:contributor "Harshvardhan J. Pandit" ;
    rdfs:isDefinedBy dpv: ;
    rdfs:subClassOf dpv:Process ;
    sw:term_status "accepted"@en ;
    skos:broader dpv:Process ;
    skos:definition "An action, activity, or method involving personal data"@en ;
    skos:inScheme dpv:process-classes ;
    skos:prefLabel "Personal Data Process"@en .

dpv:Process a rdfs:Class,
        skos:Concept ;
    dct:contributor "Harshvardhan J. Pandit" ;
    rdfs:isDefinedBy dpv: ;
    sw:term_status "accepted"@en ;
    skos:definition "An action, activity, or method"@en ;
    skos:inScheme dpv:process-classes ;
    skos:prefLabel "Process"@en .

dpv:Service a rdfs:Class,
        skos:Concept ;
    dct:contributor "Harshvardhan J. Pandit" ;
    rdfs:isDefinedBy dpv: ;
    rdfs:subClassOf dpv:Process ;
    sw:term_status "accepted"@en ;
    skos:broader dpv:Process ;
    skos:definition "A service is a process where one entity provides some benfit or assistance to another entity"@en ;
    skos:inScheme dpv:process-classes ;
    skos:prefLabel "Service"@en ;
    skos:scopeNote "Service Provider and Service Consumer reflect the roles associated with a service"@en .

<https://w3id.org/dpv> a owl:Ontology,
        profile:Profile ;
    dct:conformsTo "http://www.w3.org/2000/01/rdf-schema",
        "http://www.w3.org/2004/02/skos/core" ;
    dct:contributor "Axel Polleres",
        "Georg P. Krog",
        "Harshvardhan J. Pandit",
        "Javier Fernández" ;
    dct:created "2022-08-18"@en ;
    dct:creator "Harshvardhan J. Pandit"@en ;
    dct:description "The Data Privacy Vocabulary (DPV) provides terms (classes and properties) to represent information about processing of personal data, for example - purposes, processing operations, personal data, technical and organisational measures."@en ;
    dct:identifier "https://w3id.org/dpv" ;
    dct:license <https://www.w3.org/copyright/document-license-2023/> ;
    dct:modified "2024-01-01"@en ;
    dct:title "Data Privacy Vocabulary (DPV)"@en ;
    vann:preferredNamespacePrefix "dpv" ;
    vann:preferredNamespaceUri "https://w3id.org/dpv#" ;
    profile:hasResource dpv:serialisation-n3,
        dpv:serialisation-rdf,
        dpv:serialisation-ttl,
        <https://w3id.org/dpv/examples>,
        <https://w3id.org/dpv/guides>,
        <https://w3id.org/dpv/primer> ;
    profile:isProfileOf rdfs:,
        skos: ;
    schema:version "2" .

dpv:hasNonPersonalDataProcess a rdf:Property,
        skos:Concept ;
    dcam:rangeIncludes dpv:NonPersonalDataProcess ;
    dct:contributor "Harshvardhan J. Pandit" ;
    dct:created "2023-12-12"^^xsd:date ;
    rdfs:isDefinedBy dpv: ;
    sw:term_status "accepted"@en ;
    skos:definition "Indicates association with a Non-Personal Data Process"@en ;
    skos:inScheme dpv:process-properties ;
    skos:prefLabel "has non-personal data process"@en ;
    schema:rangeIncludes dpv:NonPersonalDataProcess .

dpv:hasPersonalDataHandling a rdf:Property,
        skos:Concept ;
    dcam:rangeIncludes dpv:PersonalDataHandling ;
    dct:contributor "Harshvardhan J. Pandit, Georg P. Krog" ;
    dct:created "2022-01-19"^^xsd:date ;
    rdfs:isDefinedBy dpv: ;
    sw:term_status "accepted"@en ;
    skos:definition "Indicates association with Personal Data Handling"@en ;
    skos:inScheme dpv:process-properties ;
    skos:prefLabel "has personal data handling"@en ;
    schema:rangeIncludes dpv:PersonalDataHandling .

dpv:hasPersonalDataProcess a rdf:Property,
        skos:Concept ;
    dcam:rangeIncludes dpv:PersonalDataProcess ;
    dct:contributor "Harshvardhan J. Pandit" ;
    dct:created "2023-12-11"^^xsd:date ;
    rdfs:isDefinedBy dpv: ;
    sw:term_status "accepted"@en ;
    skos:definition "Indicates association with a Personal Data Process"@en ;
    skos:inScheme dpv:process-properties ;
    skos:prefLabel "has personal data process"@en ;
    schema:rangeIncludes dpv:PersonalDataProcess .

dpv:hasProcess a rdf:Property,
        skos:Concept ;
    dcam:rangeIncludes dpv:Process ;
    dct:contributor "Harshvardhan J. Pandit" ;
    dct:created "2023-12-10"^^xsd:date ;
    rdfs:isDefinedBy dpv: ;
    sw:term_status "accepted"@en ;
    skos:definition "Indicates association with a Process"@en ;
    skos:inScheme dpv:process-properties ;
    skos:prefLabel "has process"@en ;
    schema:rangeIncludes dpv:Process .

dpv:hasService a rdf:Property,
        skos:Concept ;
    dcam:rangeIncludes dpv:Service ;
    dct:contributor "Harshvardhan J. Pandit" ;
    dct:created "2024-04-20"^^xsd:date ;
    rdfs:isDefinedBy dpv: ;
    sw:term_status "accepted"@en ;
    skos:definition "Indicates associated with the specified service"@en ;
    skos:inScheme dpv:process-properties ;
    skos:prefLabel "has service"@en ;
    schema:rangeIncludes dpv:Service .

dpv:serialisation-n3 a profile:ResourceDescriptor ;
    dct:conformsTo <https://www.w3.org/TeamSubmission/n3/> ;
    dct:format <https://www.iana.org/assignments/media-types/text/n3> ;
    dct:title "Data Privacy Vocabulary (DPV) - N3 serialiation" ;
    profile:hasArtifact <https://w3id.org/dpv/dpv.n3> ;
    profile:hasRole role:vocabulary .

dpv:serialisation-rdf a profile:ResourceDescriptor ;
    dct:conformsTo rdf: ;
    dct:format <https://www.iana.org/assignments/media-types/application/rdf+xml> ;
    dct:title "Data Privacy Vocabulary (DPV) - RDF/XML serialiation" ;
    profile:hasArtifact <https://w3id.org/dpv/dpv.rdf> ;
    profile:hasRole role:vocabulary .

dpv:serialisation-ttl a profile:ResourceDescriptor ;
    dct:conformsTo <https://www.w3.org/TR/turtle/> ;
    dct:format <https://www.iana.org/assignments/media-types/text/turtle> ;
    dct:title "Data Privacy Vocabulary (DPV) - Turtle serialiation" ;
    profile:hasArtifact <https://w3id.org/dpv/dpv.ttl> ;
    profile:hasRole role:vocabulary .

<https://w3id.org/dpv/examples> a profile:ResourceDescriptor ;
    dct:conformsTo <https://www.w3.org/TR/html/> ;
    dct:format <https://www.iana.org/assignments/media-types/text/html> ;
    dct:title "Examples for Data Privacy Vocabulary" ;
    profile:hasArtifact <https://w3id.org/dpv/examples> ;
    profile:hasRole role:guidance .

<https://w3id.org/dpv/guides> a profile:ResourceDescriptor ;
    dct:conformsTo <https://www.w3.org/TR/html/> ;
    dct:format <https://www.iana.org/assignments/media-types/text/html> ;
    dct:title "Guides for Data Privacy Vocabulary" ;
    profile:hasArtifact <https://w3id.org/dpv/guides> ;
    profile:hasRole role:guidance .

<https://w3id.org/dpv/primer> a profile:ResourceDescriptor ;
    dct:conformsTo <https://www.w3.org/TR/html/> ;
    dct:format <https://www.iana.org/assignments/media-types/text/html> ;
    dct:title "Primer for Data Privacy Vocabulary" ;
    profile:hasArtifact <https://w3id.org/dpv/primer> ;
    profile:hasRole role:guidance .

dpv:process-classes a skos:ConceptScheme .

dpv:process-properties a skos:ConceptScheme .

